adjustments

FOF_Tseitin.thy
@@ -1,41 +1,33 @@
 theory FOF_Tseitin
-  imports Main FOF_Base
+  imports Main FOF_Base FOF_Simplify
 begin
 
 inductive is_prop :: "('v, 'f, 'p) formula \<Rightarrow> bool" where
-Prop: "is_prop (Pred P [])" |
+Prop: "is_prop (Pred p [])" |
 And: "is_prop f1 \<Longrightarrow> is_prop f2 \<Longrightarrow> is_prop (And f1 f2)" |
 Or: "is_prop f1 \<Longrightarrow> is_prop f2 \<Longrightarrow> is_prop (Or f1 f2)" |
 Not: "is_prop f \<Longrightarrow> is_prop (Not f)"
 
-inductive is_literal :: "('v, 'f, 'p) formula \<Rightarrow> bool" where
-True: "is_literal T" |
-False: "is_literal F" |
-Prop: "is_literal (Pred p args)" |
-Equal: "is_literal (Equal t1 t2)" |
-NProp: "is_literal (Not (Pred p args))" |
-NEqual: "is_literal (Not (Equal t1 t2))" 
+inductive is_prop_literal :: "('v, 'f, 'p) formula \<Rightarrow> bool" where
+Prop: "is_prop_literal (Pred p [])" |
+NProp: "is_prop_literal (Not (Pred p []))"
 
-inductive is_nnf :: "('v, 'f, 'p) formula \<Rightarrow> bool" where
-Literal: "is_literal f \<Longrightarrow> is_nnf f" |
-And: "is_nnf f1 \<Longrightarrow> is_nnf f2 \<Longrightarrow> is_nnf (And f1 f2)" |
-Or: "is_nnf f1 \<Longrightarrow> is_nnf f2 \<Longrightarrow> is_nnf (Or f1 f2)" |
-Forall: "is_nnf f \<Longrightarrow> is_nnf (Forall v f)" |
-Exists: "is_nnf f \<Longrightarrow> is_nnf (Exists v f)"
+inductive is_prop_nnf :: "('v, 'f, 'p) formula \<Rightarrow> bool" where
+Prop: "is_prop_nnf (Pred p [])" |
+NProp: "is_prop_nnf (Not (Pred p []))" |
+And: "is_prop_nnf f1 \<Longrightarrow> is_prop_nnf f2 \<Longrightarrow> is_prop_nnf (And f1 f2)" |
+Or: "is_prop_nnf f1 \<Longrightarrow> is_prop_nnf f2 \<Longrightarrow> is_prop_nnf (Or f1 f2)"
 
-(*
-inductive is_clause :: "('v, 'f, 'p) formula \<Rightarrow> bool" where
-Literal: "is_literal f \<Longrightarrow> is_clause f" |
-Or: "is_literal f1 \<Longrightarrow> is_literal f2 \<Longrightarrow> is_clause (Or f1 f2)"
+inductive is_prop_clause :: "('v, 'f, 'p) formula \<Rightarrow> bool" where
+Literal: "is_prop_literal f \<Longrightarrow> is_prop_clause f" |
+Or: "is_prop_literal f1 \<Longrightarrow> is_prop_literal f2 \<Longrightarrow> is_prop_clause (Or f1 f2)"
 
 inductive is_cnf :: "('v, 'f, 'p) formula \<Rightarrow> bool" where
-Literal: "is_literal f \<Longrightarrow> is_cnf f" |
-And: "is_clause f1 \<Longrightarrow> is_clause f2 \<Longrightarrow> is_cnf (And f1 f2)" 
-*)
+Literal: "is_prop_literal f \<Longrightarrow> is_cnf f" |
+And: "is_prop_clause f1 \<Longrightarrow> is_prop_clause f2 \<Longrightarrow> is_cnf (And f1 f2)" 
 
 type_synonym 'p fresh = "'p set \<Rightarrow> 'p"
 type_synonym ('v, 'f, 'p) tseitin_asgnm = "'p \<times> ('v, 'f, 'p) formula"
-type_synonym ('v, 'f, 'p) tseitin_asgnm_conv = "('v, 'f, 'p) formula \<times> ('v, 'f, 'p) formula"
 
 fun tseitin_occup_var :: "('v, 'f, 'p) formula \<Rightarrow> 'p set" where
 "tseitin_occup_var (Pred p []) = {p}" |
@@ -51,29 +43,23 @@ fun tseitin_list :: "('v, 'f, 'p) formula \<Rightarrow> ('v, 'f, 'p) formula lis
 "tseitin_list (Or f1 f2) = [Or f1 f2] @ tseitin_list f1 @ tseitin_list f2" |
 "tseitin_list _ = []"
 
-definition tseitin_fresh_var :: "'p fresh \<Rightarrow> 'p set \<Rightarrow> 'p set \<times> 'p" where
-"tseitin_fresh_var \<xi> \<Sigma> = (let \<tau> = \<xi> \<Sigma> in (\<Sigma> \<union> {\<tau>}, \<tau>))"
-
-definition tseitin_assign_var :: "'p \<Rightarrow> ('v, 'f, 'p) formula \<Rightarrow> ('v, 'f, 'p) tseitin_asgnm" where
-"tseitin_assign_var \<tau> f = (\<tau>, f)"
+definition tseitin_fresh_var :: "'p fresh \<Rightarrow> 'p set \<Rightarrow> 'p \<times> 'p set" where
+"tseitin_fresh_var \<xi> \<Sigma> = (let \<tau> = \<xi> \<Sigma> in (\<tau>, \<Sigma> \<union> {\<tau>}))"
 
 fun tseitin_list_asgnm :: 
 "'p fresh \<Rightarrow> 'p set \<Rightarrow> ('v, 'f, 'p) formula list \<Rightarrow> ('v, 'f, 'p) tseitin_asgnm list" where
 "tseitin_list_asgnm \<xi> \<Sigma> [] = []" |
 "tseitin_list_asgnm \<xi> \<Sigma> (f # fs) = 
   (let fresh_var = tseitin_fresh_var \<xi> \<Sigma>;
-       assign_var = tseitin_assign_var (snd fresh_var) f
-    in [assign_var] @ tseitin_list_asgnm \<xi> (fst fresh_var) fs)"
-
-definition tseitin_conv_var :: "'p \<Rightarrow> ('v, 'f, 'p) formula" where
-"tseitin_conv_var \<tau> = Pred \<tau> []"
+       assign_var = ((fst fresh_var), f)
+    in assign_var # tseitin_list_asgnm \<xi> (snd fresh_var) fs)"
 
 fun tseitin_subst_formula ::
 "('v, 'f, 'p) formula \<Rightarrow> ('v, 'f, 'p) tseitin_asgnm list \<Rightarrow> ('v, 'f, 'p) formula" where
 "tseitin_subst_formula f [] = f" |
 "tseitin_subst_formula f (a # as) = 
   (if (f = snd a) 
-   then tseitin_conv_var (fst a)
+   then Pred (fst a) []
    else tseitin_subst_formula f as)"
 
 fun tseitin_subst_subformula :: 
@@ -97,10 +83,7 @@ fun tseitin_list_subst :: "('v, 'f, 'p) tseitin_asgnm list \<Rightarrow> ('v, 'f
   (let f' = tseitin_subst_subformula f as
     in (\<tau>, f') # tseitin_list_subst as)"
 
-fun tseitin_conv_asgnm :: 
-"('v, 'f, 'p) tseitin_asgnm \<Rightarrow> ('v, 'f, 'p) tseitin_asgnm_conv" where
-"tseitin_conv_asgnm (\<tau>, f) = (tseitin_conv_var \<tau>, f)"
-
+(*
 fun tseitin_simp_formula :: "('v, 'f, 'p) formula \<Rightarrow> ('v, 'f, 'p) formula" where
 "tseitin_simp_formula (Pred p []) = Pred p []" |
 "tseitin_simp_formula (And \<phi>1 \<phi>2) = And (tseitin_simp_formula \<phi>1) (tseitin_simp_formula \<phi>2)" |
@@ -110,6 +93,7 @@ fun tseitin_simp_formula :: "('v, 'f, 'p) formula \<Rightarrow> ('v, 'f, 'p) for
   Not (Pred p []) \<Rightarrow> Pred p []
 )" |
 "tseitin_simp_formula \<phi> = \<phi>"
+*)
 
 fun tseitin_equiv_binding :: 
 "('v, 'f, 'p) formula \<Rightarrow> ('v, 'f, 'p) formula \<Rightarrow> ('v, 'f, 'p) formula \<Rightarrow> ('v, 'f, 'p) formula" where
@@ -125,69 +109,90 @@ fun tseitin_equiv_binding ::
     in And l r'')" |
 "tseitin_equiv_binding _ l r = And l r"
 
-fun tseitin_transform_to_clause :: "('v, 'f, 'p) tseitin_asgnm_conv \<Rightarrow> ('v, 'f, 'p) formula" where
-"tseitin_transform_to_clause (\<tau>_conv, \<phi>) =
-  (let l = Imp \<tau>_conv \<phi>;
+fun tseitin_transform_to_clause :: "('v, 'f, 'p) tseitin_asgnm \<Rightarrow> ('v, 'f, 'p) formula" where
+"tseitin_transform_to_clause (\<tau>, \<phi>) =
+  (let \<tau>_conv = Pred \<tau> [];
+       l = Imp \<tau>_conv \<phi>;
        r = Imp \<phi> \<tau>_conv;
        equiv = tseitin_equiv_binding \<phi> l r
-    in tseitin_simp_formula equiv
+    in simp_formula equiv
 )"
 
 fun tseitin_get_head_var :: 
-"('v, 'f, 'p) formula \<Rightarrow> ('v, 'f, 'p) tseitin_asgnm_conv list \<Rightarrow> ('v, 'f, 'p) formula" where
-"tseitin_get_head_var (Pred p []) [] = Pred p []" |
-"tseitin_get_head_var \<phi> [] = \<phi>" |
+"('v, 'f, 'p) formula \<Rightarrow> ('v, 'f, 'p) tseitin_asgnm list \<Rightarrow> 'p" where
+"tseitin_get_head_var (Pred p []) [] = p" |
 "tseitin_get_head_var _ as = fst (hd as)"
 
-fun tseitin_conjunct_clauses :: 
-"('v, 'f, 'p) formula \<Rightarrow> ('v, 'f, 'p) formula list \<Rightarrow> ('v, 'f, 'p) formula" where
-"tseitin_conjunct_clauses (Pred p []) [] = Pred p []" |
-"tseitin_conjunct_clauses start [] = start" |
-"tseitin_conjunct_clauses start cls = fold And cls start"
+fun tseitin_get_new_vars :: "('v, 'f, 'p) tseitin_asgnm list \<Rightarrow> 'p set" where
+"tseitin_get_new_vars [] = {}" |
+"tseitin_get_new_vars (a # as) = {fst a} \<union> tseitin_get_new_vars as"
 
-fun tseitin_expansion :: "'p fresh \<Rightarrow> ('v, 'f, 'p) formula \<Rightarrow> ('v, 'f, 'p) formula" where
-"tseitin_expansion \<xi> \<phi> = 
-  (let \<Sigma> = tseitin_occup_var \<phi>;
-       list = tseitin_list \<phi>;
+definition tseitin_decompose ::
+"'p fresh \<Rightarrow> 'p set \<Rightarrow> ('v, 'f, 'p) formula \<Rightarrow> 'p \<times> ('v, 'f, 'p) formula list \<times> 'p set" where
+"tseitin_decompose \<xi> \<Sigma> \<phi> = 
+  (let list = tseitin_list \<phi>;
        list_asgnm = tseitin_list_asgnm \<xi> \<Sigma> list;
        list_subst = tseitin_list_subst list_asgnm;
-       list_conv = map tseitin_conv_asgnm list_subst;
-       list_clause = map tseitin_transform_to_clause list_conv;
-       head_var = tseitin_get_head_var \<phi> list_conv;
-       tseitin_\<phi>_cnf = tseitin_conjunct_clauses head_var list_clause
-    in tseitin_\<phi>_cnf
+       list_clause = map tseitin_transform_to_clause list_subst;
+       head_var = tseitin_get_head_var \<phi> list_asgnm;
+       new_vars = tseitin_get_new_vars list_asgnm
+    in (head_var, list_clause, new_vars)
 )"
+
+fun tseitin_conjunct_clauses :: 
+"'p \<Rightarrow> ('v, 'f, 'p) formula list \<Rightarrow> ('v, 'f, 'p) formula" where
+"tseitin_conjunct_clauses p [] = (Pred p [])" |
+"tseitin_conjunct_clauses p cls = fold And cls (Pred p [])"
+
+definition tseitin_expansion :: "'p fresh \<Rightarrow> ('v, 'f, 'p) formula \<Rightarrow> ('v, 'f, 'p) formula" where
+"tseitin_expansion \<xi> \<phi> = 
+  (let (\<tau>, \<C>, \<Sigma>') = tseitin_decompose \<xi> (tseitin_occup_var \<phi>) \<phi>
+    in tseitin_conjunct_clauses \<tau> \<C>
+)"
+
+lemma tseitin_Prop_empty_args:
+  fixes fresh :: "'p set \<Rightarrow> 'p"
+  assumes "\<And>\<P>. finite \<P> \<Longrightarrow> fresh \<P> \<notin> \<P>"
+  shows "tseitin_expansion fresh (Pred p []) = Pred p []" 
+proof -
+  have list_asgnm: "tseitin_list_asgnm fresh {p} [] = []"
+    by simp
+  have to_clause: "map tseitin_transform_to_clause [] = []"
+    by simp
+  have decompose: "tseitin_decompose fresh {p} (Pred p []) = (p, [], {})"
+    unfolding tseitin_decompose_def Let_def tseitin_list.simps list_asgnm
+              tseitin_get_head_var.simps tseitin_list_subst.simps
+              to_clause tseitin_get_new_vars.simps
+    by simp
+  show ?thesis
+    unfolding tseitin_expansion_def tseitin_occup_var.simps decompose Let_def
+    by simp
+qed 
 
 theorem eval_tseitin_equiv_eval:
   fixes fresh :: "'p set \<Rightarrow> 'p" and \<phi> :: "('v, 'f, 'p) formula"
   assumes "\<And>\<P>. finite \<P> \<Longrightarrow> fresh \<P> \<notin> \<P>"
-  assumes "is_nnf \<phi>"
-  assumes "is_prop \<phi>"
-  shows "(\<exists>pI. eval_formula (tseitin_expansion fresh \<phi>) vI fI pI) \<longleftrightarrow> (\<exists>pI. eval_formula \<phi> vI fI pI)"
-proof -
-  have "is_prop \<phi>" using assms by simp
-  then show ?thesis
-  proof (induction \<phi> rule: is_prop.induct)
-    case (Prop P)
-    then show ?case
-    proof
-      assume "\<exists>pI. eval_formula (tseitin_expansion fresh (Pred P [])) vI fI pI"
-      then show "\<exists>pI. eval_formula (Pred P []) vI fI pI"
-        by simp
-    next
-      assume "\<exists>pI. eval_formula (Pred P []) vI fI pI"
-      then show "\<exists>pI. eval_formula (tseitin_expansion fresh (Pred P [])) vI fI pI"
-        by simp
-    qed
-  next
-    case (And f1 f2)
-    then show ?case sorry
-  next
-    case (Or f1 f2)
-    then show ?case sorry
-  next
-    case (Not f)
-    then show ?case sorry
-  qed
+  assumes "is_prop_nnf \<phi>"
+  shows "(\<exists>pI. eval_formula (tseitin_expansion fresh \<phi>) vI fI pI) 
+    \<longleftrightarrow> (\<exists>pI. eval_formula \<phi> vI fI pI)"
+  (is "?LHS \<longleftrightarrow> ?RHS")
+  using \<open>is_prop_nnf \<phi>\<close>
+proof (induction \<phi> rule: is_prop_nnf.induct)
+  case (Prop p)
+  then show ?case
+    by (simp add: assms(1) tseitin_Prop_empty_args)
+next
+  case (NProp p)
+  then show ?case
+    sorry
+next
+  case (And f1 f2)
+  then show ?case
+    sorry
+next
+  case (Or f1 f2)
+  then show ?case
+    sorry
 qed
+
 end
